src/lib/kuiper/Kuiper.Approximates.F64.fsti
@@ -4,3 +4,5 @@ open Kuiper
 open Kuiper.Approximates.Base
 
 instance val real_like_f64 : real_like f64
+
+instance val floating_real_like_f64 : floating_real_like f64
