src/lib/kuiper/Kuiper.Approximates.fst
@@ -14,13 +14,13 @@ let to_real_seq_is_approx (#a:Type) {| scalar a, d : real_like a |}
     Classical.forall_intro aux
 
 let real_seq_sum_append
-  (r1 r2 : seq Real.real)
+  (r1 r2 : seq real)
   : Lemma (ensures real_seq_sum (r1 `Seq.append` r2) == real_seq_sum r1 +. real_seq_sum r2)
           (decreases Seq.length r1)
   = lemma_seq_fold_left_sum 0.0R (+.) r1 r2
 
 let seq_approximates_append (#a:Type) {| scalar a, real_like a |}
-  (s1 s2 : a) (r1 r2 : seq Real.real)
+  (s1 s2 : a) (r1 r2 : seq real)
   : Lemma (requires s1 `approximates` real_seq_sum r1 /\ s2 `approximates` real_seq_sum r2)
           (ensures (s1 `add` s2) `approximates` real_seq_sum (r1 `Seq.append` r2))
   = a_add s1 s2 (real_seq_sum r1) (real_seq_sum r2);
