src/lib/kuiper/Kuiper.Approximates.fsti
@@ -44,22 +44,22 @@ let ( |~> ) #pt #rt #mt {| has_pts_to pt rt, can_approximate rt mt |}
   exists* (v : rt). p |-> v ** pure (v %~ m)
 
 instance real_like_can_approximate (#a:Type) (_ : scalar a) (_ : real_like a)
-  : can_approximate a Real.real = {
+  : can_approximate a real = {
   approximates = v_approximates;
 }
 
 let seq_approximates (#a:Type) {| scalar a, real_like a |}
-  (s : seq a) (r : seq Real.real) : prop
+  (s : seq a) (r : seq real) : prop
   = Seq.length s == Seq.length r /\
     (forall i. i < len s ==> (s @! i) %~ (r @! i))
 
 instance seq_real_like_can_approximate (#a:Type) {| scalar a, real_like a |}
-  : can_approximate (seq a) (seq Real.real) = {
+  : can_approximate (seq a) (seq real) = {
   approximates = seq_approximates;
 }
 
 let to_real_seq (#a:Type) {| scalar a, real_like a |}
-  (s : seq a) : GTot (seq Real.real)
+  (s : seq a) : GTot (seq real)
   = Seq.init_ghost (Seq.length s) (fun i -> to_real (s @! i))
 
 val to_real_seq_is_approx (#a:Type) {| scalar a, real_like a |}
@@ -67,14 +67,14 @@ val to_real_seq_is_approx (#a:Type) {| scalar a, real_like a |}
   : Lemma (s %~ to_real_seq s)
           [SMTPat (seq_approximates s (to_real_seq s))]
 
-let real_seq_sum (r : seq Real.real) : Real.real
+let real_seq_sum (r : seq real) : real
   = seq_fold_left (+.) 0.0R r
 
 val real_seq_sum_append
-  (r1 r2 : seq Real.real)
+  (r1 r2 : seq real)
   : Lemma (real_seq_sum (r1 `Seq.append` r2) == real_seq_sum r1 +. real_seq_sum r2)
 
 val seq_approximates_append (#a:Type) {| scalar a, real_like a |}
-  (s1 s2 : a) (r1 r2 : seq Real.real)
+  (s1 s2 : a) (r1 r2 : seq real)
   : Lemma (requires s1 %~ real_seq_sum r1 /\ s2 %~ real_seq_sum r2)
           (ensures (s1 `add` s2) %~ real_seq_sum (r1 `Seq.append` r2))
